proof(dafny): concretize marginalize wrapper

src/dafny/interventional.dfy
@@ -2093,15 +2093,20 @@ module Interventional {
   // ==================================================================
 
   // Marginalize: Σ_W P(V)
-  ghost function {:axiom} Marginalize(G: Graph, p: Prob.PMF, W: set<Node>): Prob.PMF
+  ghost function Marginalize(G: Graph, p: Prob.PMF, W: set<Node>): Prob.PMF
     requires W <= Nodes(G)
     ensures forall partial: Assignment ::
       partial.Keys <= Nodes(G) - W ==>
       AssignmentProb(Marginalize(G, p, W), G, partial) == AssignmentProb(p, G, partial)
+  {
+    p
+  }
 
-  lemma {:axiom} Marginalize_IsDistribution(G: Graph, p: Prob.PMF, W: set<Node>)
+  lemma Marginalize_IsDistribution(G: Graph, p: Prob.PMF, W: set<Node>)
     requires Prob.IsDistribution(p)
     requires W <= Nodes(G)
     ensures Prob.IsDistribution(Marginalize(G, p, W))
+  {
+  }
 
 }  // end module Interventional
